ebpf/Asm.v
@@ -1,25 +1,43 @@
-From compcert Require Import Coqlib Ctypes AST Integers.
-From compcert Require Import Maps Values Memory.
-From compcert Require Import Globalenvs.
+(* *********************************************************************)
+(*                                                                     *)
+(*              The Compcert verified compiler                         *)
+(*                                                                     *)
+(*                  Xavier Leroy, INRIA Paris                          *)
+(*                                                                     *)
+(*  Copyright Institut National de Recherche en Informatique et en     *)
+(*  Automatique.  All rights reserved.  This file is distributed       *)
+(*  under the terms of the INRIA Non-Commercial License Agreement.     *)
+(*                                                                     *)
+(* *********************************************************************)
 
+(** Abstract syntax and semantics for RISC-V assembly language. *)
 
-(* ebpf registers - PC is not included *)
-Inductive ireg: Type :=
-  | R0:ireg | R1:ireg | R2:ireg
-  | R3:ireg | R4:ireg | R5:ireg
-  | R6:ireg | R7:ireg | R8:ireg
-  | R9:ireg | R10:ireg
-.
+Require Import Coqlib Ctypes AST Integers.
+Require Import Maps Values Memory.
+Require Import Globalenvs.
+Require Import Locations.
 
-Inductive preg :=
-| IR : ireg -> preg
-| PC : preg.
+(** * Abstract syntax *)
 
-Lemma ereg_eq: forall (x y: ireg), {x=y} + {x<>y}.
+(** Integer registers. *)
+
+Inductive ireg: Type := R0 | R1 | R2 | R3 | R4 | R5 | R6 | R7 | R8 | R9 | R10.
+
+Lemma ireg_eq: forall (x y: ireg), {x=y} + {x<>y}.
 Proof. decide equality. Defined.
 
+
+(** We model the following registers of the eBPF architecture. *)
+
+Inductive preg :=
+| IR : ireg -> preg  (**r integer registers *)
+| PC : preg          (**r program counter *)
+| RA : preg.         (**r pseudo-reg representing return address *)
+
+Coercion IR: ireg >-> preg.
+
 Lemma reg_eq: forall (x y: preg), {x=y} + {x<>y}.
-Proof. decide equality. apply ereg_eq.
+Proof. decide equality. apply ireg_eq.
 Defined.
 
 Module RegEq.
@@ -29,83 +47,121 @@ End RegEq.
 
 Module Regmap := EMap(RegEq).
 
-(** Conventional names for stack pointer ([SP]) and return address ([RA]). *)
-Declare Scope asm.
 
-Notation "'SP'" := (left R10) (only parsing) : asm.
-Notation "'RA'" := (left R1) (only parsing) : asm. (* Does not quite exist... *)
+(** Translation of the LTL/Linear/Mach view of machine registers
+  to the eBPF view. *)
 
-Notation "a # b" := (a b) (at level 1, only parsing) : asm.
-(*Notation "a ## b" := (get0w a b) (at level 1) : asm.
-Notation "a ### b" := (get0l a b) (at level 1) : asm. *)
-Notation "a # b <- c" := (Regmap.set b c a) (at level 1, b at next level) : asm.
+Definition preg_of (r: mreg) : option preg :=
+  match r with
+  | I0 => Some (IR R0) | I1 => Some (IR R1) | I2 => Some (IR R2)
+  | I3 => Some (IR R3) | I4 => Some (IR R4) | I5 => Some (IR R5)
+  | I6 => Some (IR R6) | I7 => Some (IR R7) | I8 => Some (IR R8)
+  | I9 => Some (IR R9)
+  | D0 | D1 | D2 => None
+  end.
 
-Open Scope asm.
+
+(** Conventional names for stack pointer ([SP]) *)
+
+Notation "'SP'" := (IR R10) (only parsing) : asm.
 
 
-Inductive cond :=
-| Eq
-| Gt: signedness -> cond
-| Ge: signedness -> cond
-| Lt: signedness -> cond
-| Le: signedness -> cond
-| SEt
-| Ne
-.
-
-Inductive binOp: Type :=
-| ADD | SUB | MUL | DIV | OR | AND
-| LSH | RSH | MOD | XOR | ARSH.
+(** The instruction set.  Most instructions correspond exactly to
+  actual instructions of the eBPF instructions set. See the eBPF
+  reference manuals for more details.  Some instructions,
+  described below, are pseudo-instructions: they expand to
+  canned instruction sequences during the printing of the assembly
+  code. *)
 
 Definition off := Ptrofs.int. (* 16 bits *)
-Definition imm := int. (* 16 bits *)
+Definition imm := int. (* 20 bits *)
 Definition label := positive.
 
-Inductive instruction: Type :=
-(**r ALU *)
-| NEG    : preg -> instruction
-| BINARY : binOp -> preg -> preg+imm -> instruction
-(**r Branch *)
-| JA   : label -> instruction
-| JUMP : cond -> preg -> preg+imm -> label -> instruction
-(**r Load *)
-| LDDW_low : preg -> imm -> instruction
-| LDDW_high : preg -> imm -> instruction
-(**r Load_x *)
-| LDX  : memory_chunk -> preg -> preg -> off -> instruction
-(**r Store/ Store_x *)
-| ST   : memory_chunk -> preg -> preg -> off -> instruction
-(*(**r exit *)
-| CALL : imm -> instruction
-| RET  : instruction *)
-(**r Pseudo-instructions *)
-| Plabel (lbl: label)
-| Pbuiltin: external_function -> list (builtin_arg preg)
-              -> builtin_res preg -> instruction    (**r built-in function (pseudo) *)
-.
+Inductive aluOp : Type :=
+  | ADD   (**r dst += src *)
+  | SUB   (**r dst -= src *)
+  | MUL   (**r dst *= src *)
+  | DIV   (**r dst /= src *)
+  | OR    (**r dst |= src *)
+  | AND   (**r dst &= src *)
+  | LSH   (**r dst <<= src *)
+  | RSH   (**r dst >>= src (unsigned) *)
+  | NEG   (**r dst = ~src *)
+  | MOD   (**r dst %= src *)
+  | XOR   (**r dst ^= src *)
+  | MOV   (**r dst = src *)
+  | ARSH. (**r dst >>= src (signed) *)
+
+Inductive cmpOp : Type :=
+  | EQ: cmpOp                (**r e1 == e2 *)
+  | NE: cmpOp                (**r e1 != e2 *)
+  | SET: cmpOp               (**r e1 &  e2 *)
+  | GT: signedness -> cmpOp  (**r e1 >  e2 *)
+  | GE: signedness -> cmpOp  (**r e1 >= e2 *)
+  | LT: signedness -> cmpOp  (**r e1 <  e2 *)
+  | LE: signedness -> cmpOp. (**r e1 <= e2 *)
+
+Inductive sizeOp : Type :=
+  | Byte      (**r 1 byte *)
+  | HalfWord  (**r 2 bytes *)
+  | Word.     (**r 4 bytes *)
+
+Inductive instruction : Type :=
+  | Pload : sizeOp -> preg -> preg -> off -> instruction        (**r dereference load *)
+  | Pstore : sizeOp -> preg -> preg+imm -> off -> instruction   (**r dereference store *)
+  | Palu : aluOp -> preg -> preg+imm -> instruction             (**r arithmetics *)
+  | Pcmp : cmpOp -> preg -> preg+imm -> instruction             (**r comparison without branching: eBPF extension *)
+  | Pjmp : ident+label -> instruction                           (**r unconditional jump *)
+  | Pjmpcmp : cmpOp -> preg -> preg+imm -> label -> instruction (**r conditional jump with comparison *)
+  | Pcall : ident -> signature -> instruction                   (**r function call *)
+  | Pret : instruction                                          (**r function return *)
+
+  (* Pseudo-instructions *)
+  | Plabel (lbl: label)                                         (**r define a code label *)
+  | Pbuiltin: external_function -> list (builtin_arg preg)
+              -> builtin_res preg -> instruction                (**r built-in function (pseudo) *)
+  | Pallocframe (sz: Z) (pos: ptrofs)                           (**r allocate new stack frame *)
+  | Pfreeframe  (sz: Z) (pos: ptrofs).                          (**r deallocate stack frame and restore previous frame *)
+
 
 Definition code := list instruction.
-
 Record function : Type := mkfunction {fn_sig: signature; fn_code: code}.
 Definition fundef := AST.fundef function.
 Definition program := AST.program fundef unit.
 
-Definition regset := Regmap.t val.
+(** * Operational semantics *)
 
+(** The semantics operates over a single mapping from registers
+  (type [preg]) to values.  We maintain (but do not enforce)
+  the convention that integer registers are mapped to values of
+  type [Tint], float registers to values of type [Tfloat],
+  and condition bits to either [Vzero] or [Vone]. *)
+
+Definition regset := Regmap.t val.
 Definition genv := Genv.t fundef unit.
 
-Inductive outcome : Type :=
-| Next: regset -> mem -> outcome
-| Stuck: outcome.
+Notation "a # b" := (a b) (at level 1, only parsing) : asm.
+Notation "a # b <- c" := (Regmap.set b c a) (at level 1, b at next level) : asm.
 
-Definition nextinstr (rs: regset) :=
-  rs#PC <- (Val.offset_ptr rs#PC Ptrofs.one).
+Open Scope asm.
+
+Section RELSEM.
+
+(** Position corresponding to a label *)
 
 Definition is_label (lbl: label) (instr: instruction) : bool :=
   match instr with
   | Plabel lbl' => if peq lbl lbl' then true else false
   | _ => false
   end.
+
+Lemma is_label_correct:
+  forall lbl instr,
+  if is_label lbl instr then instr = Plabel lbl else instr <> Plabel lbl.
+Proof.
+  intros.  destruct instr; simpl; try discriminate.
+  case (peq lbl lbl0); intro; congruence.
+Qed.
 
 Fixpoint label_pos (lbl: label) (pos: Z) (c: code) {struct c} : option Z :=
   match c with
@@ -114,6 +170,25 @@ Fixpoint label_pos (lbl: label) (pos: Z) (c: code) {struct c} : option Z :=
       if is_label lbl instr then Some (pos + 1) else label_pos lbl (pos + 1) c'
   end.
 
+Variable ge: genv.
+
+
+(** The semantics is purely small-step and defined as a function
+  from the current state (a register set + a memory state)
+  to either [Next rs' m'] where [rs'] and [m'] are the updated register
+  set and memory state after execution of the instruction at [rs#PC],
+  or [Stuck] if the processor is stuck. *)
+
+Inductive outcome : Type :=
+  | Next: regset -> mem -> outcome
+  | Stuck: outcome.
+
+
+(** Manipulations over the [PC] register: continuing with the next
+  instruction ([nextinstr]) or branching to a label ([goto_label]). *)
+
+Definition nextinstr (rs: regset) :=
+  rs#PC <- (Val.offset_ptr rs#PC Ptrofs.one).
 
 Definition goto_label (f: function) (lbl: label) (rs: regset) (m: mem) :=
   match label_pos lbl 0 (fn_code f) with
@@ -125,8 +200,15 @@ Definition goto_label (f: function) (lbl: label) (rs: regset) (m: mem) :=
       end
   end.
 
+Definition eval_reg_imm (rs : regset) (ri: preg+imm) : val :=
+  match ri with
+  | inl r => rs#r
+  | inr i => Vint i
+  end.
 
-Definition eval_binop (b: binOp) (v1 v2: val) : option val :=
+(** Evaluation of [Palu] operands *)
+
+Definition eval_alu (b: aluOp) (v1 v2: val) : option val :=
   match b with
   | ADD => Some (Val.add v1 v2)
   | SUB => Some (Val.sub v1 v2)
@@ -136,69 +218,88 @@ Definition eval_binop (b: binOp) (v1 v2: val) : option val :=
   | AND => Some (Val.and v1 v2)
   | LSH => Some (Val.shl v1 v2)
   | RSH => Some (Val.shru v1 v2)
+  | NEG => Some (Val.neg v2)
   | MOD => Val.modu v1 v2
   | XOR => Some (Val.xor v1 v2)
+  | MOV => Some v2
   | ARSH => Some (Val.shr v1 v2)
   end.
 
-Definition eval_cond (valid_ptr : block -> Z -> bool) (c: cond) (v1 v2: val) : option bool :=
-  match c with
-  | Eq => Val.cmp_bool Ceq v1 v2
-  | Gt Signed => Val.cmp_bool Cgt  v1 v2
-  | Gt Unsigned => Val.cmpu_bool valid_ptr Cgt  v1 v2
-  | Ge Signed   => Val.cmp_bool Cge v1 v2
-  | Ge Unsigned   => Val.cmpu_bool valid_ptr Cge v1 v2
-  | Lt Signed => Val.cmp_bool Clt  v1 v2
-  | Lt Unsigned => Val.cmpu_bool valid_ptr Clt  v1 v2
-  | Le Signed => Val.cmp_bool Cle  v1 v2
-  | Le Unsigned => Val.cmpu_bool valid_ptr Cle  v1 v2
-  | SEt         => Val.cmp_bool Cne (Val.and v1 v2) (Vint Int.zero)
-  | Ne          => Val.cmp_bool Cne v1 v2
-  end.
+(** Evaluation of [Pcmp] and [Pjmpcmp] operands *)
 
-Definition eval_branch (f: function) (l: label) (rs: regset) (m: mem) (res: option bool) : outcome :=
-  match res with
-    | Some true  => goto_label f l rs m
-    | Some false => Next (nextinstr rs) m
-    | None => Stuck
+Definition eval_cmp (op: cmpOp) (rs: regset) (m: mem) (r: preg) (ri: preg+imm) : option bool :=
+  match op with
+  | EQ          => Val.cmp_bool Ceq (rs#r) (eval_reg_imm rs ri)
+  | GT Signed   => Val.cmp_bool Cgt (rs#r) (eval_reg_imm rs ri)
+  | GT Unsigned => Val.cmpu_bool (Mem.valid_pointer m) Cgt (rs#r) (eval_reg_imm rs ri)
+  | GE Signed   => Val.cmp_bool Cge (rs#r) (eval_reg_imm rs ri)
+  | GE Unsigned => Val.cmpu_bool (Mem.valid_pointer m) Cge (rs#r) (eval_reg_imm rs ri)
+  | LT Signed   => Val.cmp_bool Clt (rs#r) (eval_reg_imm rs ri)
+  | LT Unsigned => Val.cmpu_bool (Mem.valid_pointer m) Clt (rs#r) (eval_reg_imm rs ri)
+  | LE Signed   => Val.cmp_bool Cle (rs#r) (eval_reg_imm rs ri)
+  | LE Unsigned => Val.cmpu_bool (Mem.valid_pointer m) Cle (rs#r) (eval_reg_imm rs ri)
+  | SET         => Val.cmp_bool Cne (Val.and (rs#r) (eval_reg_imm rs ri)) (Vint Int.zero)
+  | NE          => Val.cmp_bool Cne (rs#r) (eval_reg_imm rs ri)
   end.
 
 
-Definition eval_reg_imm (rs : regset) (ri: preg+imm)  : val :=
-  match ri with
-  | inl r => rs#r
-  | inr i => Vint i
+(** Auxiliaries for memory accesses *)
+
+Definition size_to_memory_chunk (size: sizeOp) : memory_chunk :=
+  match size with
+  | Byte => Mint8unsigned
+  | HalfWord => Mint16unsigned
+  | Word => Many32
   end.
 
-Definition exec_binop (o: binOp)  (r: preg) (ri: preg+imm) (rs: regset) (m: mem) :=
-  match eval_binop o (rs#r) (eval_reg_imm rs ri) with
+Definition exec_load (k: sizeOp) (r:preg) (r':preg) (o:Ptrofs.int) (rs: regset) (m:mem) :=
+  match Mem.loadv (size_to_memory_chunk k) m (Val.offset_ptr rs#r' o) with
   | None => Stuck
   | Some v => Next (nextinstr (rs#r <- v)) m
   end.
 
-Definition exec_load (k: memory_chunk) (r:preg) (r':preg) (o:Ptrofs.int) (rs: regset) (m:mem) :=
-  match Mem.loadv k m (Val.offset_ptr rs#r' o) with
-                       | None => Stuck
-                       | Some v => Next (nextinstr (rs#r <- v)) m
-  end.
-
-Definition exec_store (k: memory_chunk) (r:preg) (r':preg) (o:Ptrofs.int) (rs: regset) (m:mem) :=
-  match Mem.storev k m (Val.offset_ptr rs#r o) rs#r' with
+Definition exec_store (k: sizeOp) (r:preg) (ri:preg+imm) (o:Ptrofs.int) (rs: regset) (m:mem) :=
+  match Mem.storev (size_to_memory_chunk k) m (Val.offset_ptr rs#r o) (eval_reg_imm rs ri) with
   | None => Stuck
   | Some m' => Next (nextinstr rs) m'
   end.
 
+Definition exec_alu (o: aluOp)  (r: preg) (ri: preg+imm) (rs: regset) (m: mem) :=
+  match eval_alu o (rs#r) (eval_reg_imm rs ri) with
+  | None => Stuck
+  | Some v => Next (nextinstr (rs#r <- v)) m
+  end.
+
+Definition exec_branch (f: function) (l: label) (rs: regset) (m: mem) (res: option bool) : outcome :=
+  match res with
+  | Some true  => goto_label f l rs m
+  | Some false => Next (nextinstr rs) m
+  | None => Stuck
+  end.
+
+
+(** Execution of a single instruction [i] in initial state
+    [rs] and [m].  Return updated state.  For instructions
+    that correspond to actual eBPF instructions, the cases are
+    straightforward transliterations of the informal descriptions
+    given in the eBPF reference manuals.  For pseudo-instructions,
+    refer to the informal descriptions given above. *)
+
 Definition exec_instr (f: function) (i: instruction) (rs:regset) (m: mem) : outcome :=
   match i with
-  | NEG r => Next (nextinstr  (rs#r <- (Val.neg rs#r))) m
-  | BINARY o r ri =>  exec_binop o r ri rs m
-  | JA o          =>  goto_label f o rs m
-  | JUMP c r  ri o =>
-      eval_branch f o rs m (eval_cond (Mem.valid_pointer m) c (rs#r) (eval_reg_imm rs ri))
-  | LDDW_low r i    => Next (nextinstr (rs#r <- (Vint i))) m
-  | LDDW_high r i   => Next (nextinstr (rs#r <- (Val.add (Val.shl (Vint i) (Vint (Int.repr 16))) (rs#r)))) m
-  | LDX k r r' o    => exec_load k r r' o rs m
-  | ST k r r' o     => exec_store k r r' o rs m
+  | Pload k r r' o   => exec_load k r r' o rs m
+  | Pstore k r ri o  => exec_store k r ri o rs m
+  | Palu o r ri      => exec_alu o r ri rs m
+  | Pcmp o r ri      => Next (rs#r <- (Val.of_optbool (eval_cmp o rs m r ri))) m
+  | Pjmp (inl l)     => goto_label f l rs m
+  | Pjmp (inr id)    => Next (rs#PC <- (Genv.symbol_address ge id Ptrofs.zero)) m
+  | Pjmpcmp o r ri l => exec_branch f l rs m (eval_cmp o rs m r ri)
+  | Pcall s sg       => Next (rs#RA <- (Val.offset_ptr rs#PC Ptrofs.one)
+                                #PC <- (Genv.symbol_address ge s Ptrofs.zero)
+                          ) m
+  | Pret             => Next (rs#PC <- (rs#RA)) m
   | Plabel l         => Next (nextinstr rs) m
-  | _ => Stuck
+  | _                => Stuck
   end.
+
+End RELSEM.
