ebpf/Stacklayout.v
@@ -16,17 +16,33 @@ Require Import Coqlib.
 Require Import Separation.
 Require Import Bounds.
 
-Local Open Scope sep_scope.
+(** The general shape of activation records is as follows,
+  from bottom (lowest offsets) to top:
+- Space for outgoing arguments to function calls.
+- Pointer to activation record of the caller.
+- Saved return address into caller.
+- Local stack slots.
+- Saved values of callee-save registers used by the function.
+- Space for the stack-allocated data declared in Cminor.
+
+The [frame_env] compilation environment records the positions of
+the boundaries between areas in the frame part.
+
+The stack pointer is kept 16-aligned.
+*)
 
 Definition fe_ofs_arg := 0.
 
+(** Computation of the frame environment from the bounds of the current
+  function. *)
+
 Definition make_env (b: bounds) : frame_env :=
   let w := if Archi.ptr64 then 8 else 4 in
-  let olink := align (4 * b.(bound_outgoing)) w in  (* back link *)
-  let oretaddr := olink + w in                      (* return address *)
-  let ocs := oretaddr + w in                        (* callee-saves *)
-  let ol :=  align (size_callee_save_area b ocs) 8 in (* locals *)
-  let ostkdata := align (ol + 4 * b.(bound_local)) 8 in (* stack data *)
+  let olink := align (4 * b.(bound_outgoing)) w in         (* back link *)
+  let oretaddr := olink + w in                             (* return address *)
+  let ocs := oretaddr + w in                               (* callee-saves *)
+  let ol := align (size_callee_save_area b ocs) 8 in       (* locals *)
+  let ostkdata := align (ol + 4 * b.(bound_local)) 8 in    (* stack data *)
   let sz := align (ostkdata + b.(bound_stack_data)) 16 in
   {| fe_size := sz;
      fe_ofs_link := olink;
